soundness of bidirectional typing

theories/Typing.v
@@ -18,7 +18,7 @@ Open Scope subst_scope.
 Definition Ax (l : level) : level :=
   ty (match l with 
   | prop => 0
-  | ty i => (i + 1)
+  | ty i => S i
   end).
 
 Definition Ru (l1 l2 : level) : level := 
