theories/TypeChecking.v
@@ -1,0 +1,400 @@
+
+From Stdlib Require Import Utf8 List Arith Bool Lia Wellfounded.Inverse_Image Wellfounded.Inclusion.
+From TypedConfluence.autosubst
+Require Import core unscoped AST SubstNotations RAsimpl AST_rasimpl.
+From TypedConfluence Require Import Util BasicAST Weakenings Contexts Typing BasicMetaTheory Confluence ConversionChecking. (*  Env Inst. *)
+From Stdlib Require Import Setoid Morphisms Relation_Definitions.
+Require Import Stdlib.Program.Equality.
+Import CombineNotations.
+
+
+Inductive cterm : Type := 
+| cann : cterm -> cterm -> cterm 
+| cvar : nat -> cterm 
+| cSort : level -> cterm 
+
+| cPi : cterm -> cterm -> cterm 
+| capp : cterm -> cterm -> cterm 
+| clam : cterm -> cterm 
+
+| cNat : cterm
+| czero : cterm 
+| csucc : cterm -> cterm
+| crec : cterm -> cterm -> cterm -> cterm -> cterm.
+
+Reserved Notation "Γ ⊢< l > M ⇒ T ↣ t" (at level 50, l, M, T, t at next level).
+Reserved Notation "Γ ⊢< l > M ⇐ T ↣ t" (at level 50, l, M, T, t at next level).
+
+
+Definition box_if_prop l t := 
+    match l with 
+    | prop => box 
+    | ty _ => t 
+    end.
+
+Definition app_box t u := 
+    match t with 
+    | box => box 
+    | _ => app prop prop box box t u
+    end.
+
+Definition lam_box t := 
+    match t with 
+    | box => box 
+    | _ => lam prop prop box box t
+    end.
+
+Definition rec_box l P p_zero p_succ k := 
+    match l with 
+    | prop => box 
+    | _ => rec l P p_zero p_succ k
+    end.
+
+
+
+Inductive infer : ctx -> level -> cterm → term -> term → Prop :=
+| infer_var Γ x l A :
+    nth_error Γ x = Some (l , A) →
+    Γ ⊢< l > cvar x ⇒ ((plus (S x)) ⋅ A) ↣ box_if_prop l (var x)
+
+| infer_Sort Γ l : 
+    Γ ⊢< Ax (Ax l) > cSort l ⇒ Sort (Ax l) ↣ Sort l
+
+| infer_pi Γ i j T U MA MB A B : 
+    Γ ⊢< Ax i > MA ⇒ T ↣ A -> 
+    T -->> Sort i ->
+    Γ ,, (i , A) ⊢< Ax j > MB ⇒ U ↣ B -> 
+    U -->> Sort j ->
+    Γ ⊢< Ax (Ru i j) > cPi MA MB ⇒ Sort (Ru i j) ↣ Pi i j A B
+
+| infer_app Γ l i j T Mt Mu t u A B :
+    Γ ⊢< l > Mt ⇒ T ↣ t -> 
+    T -->> Pi i j A B -> 
+    Γ ⊢< i > Mu ⇐ A ↣ u -> 
+    Γ ⊢< j > capp Mt Mu ⇒ B <[ u..] ↣ app_box t u
+
+| infer_Nat Γ : 
+    Γ ⊢< ty 1 > cNat ⇒ Sort (ty 0) ↣ Nat
+
+| infer_zero Γ : 
+    Γ ⊢< ty 0 > czero ⇒ Nat ↣ zero
+
+| infer_succ Γ Mt t l T :
+    Γ ⊢< l > Mt ⇒ T ↣ t -> 
+    T -->> Nat ->
+    Γ ⊢< ty 0 > csucc Mt ⇒ Nat ↣ succ t
+
+| infer_rec Γ MP P Mp_zero p_zero Mp_succ p_succ Mk k l l' T :
+    Γ ,, (ty 0, Nat) ⊢< l' > MP ⇒ T ↣ P -> 
+    T -->> Sort l ->
+    Γ ⊢< l > Mp_zero ⇐ P <[ zero ..] ↣ p_zero ->
+    Γ ,, (ty 0 , Nat) ,, (l , P) ⊢< l > Mp_succ ⇐ P <[ (succ (var 1)) .: (shift >> (shift >> var)) ] ↣ p_succ -> 
+    Γ ⊢< ty 0 > Mk ⇐ Nat ↣ k ->
+    Γ ⊢< l > crec MP Mp_zero Mp_succ Mk ⇒ P <[ k ..] ↣ rec_box l P p_zero p_succ k
+
+| infer_ann Γ MA Mt t l A T i :
+    Γ ⊢< l > MA ⇒ T ↣ A ->
+    T -->> Sort i ->
+    Γ ⊢< i > Mt ⇐ A ↣ t -> 
+    Γ ⊢< i > cann Mt MA ⇒ A ↣ t
+
+with check : ctx -> level -> cterm -> term → term → Prop :=
+| check_conv Γ Mt t l l' T T' U U' :
+    Γ ⊢< l > Mt ⇒ T ↣ t -> 
+    l = l' ->
+    T -->> T' -> nf T' -> 
+    U -->> U' -> nf U' -> 
+    T' = U' ->
+    Γ ⊢< l' > Mt ⇐ U ↣ t 
+    
+| check_lam Γ l Mt t T i j A B :
+    T -->> Pi i j A B ->
+    Γ ,, (i, A) ⊢< j > Mt ⇐ B ↣ t -> 
+    Γ ⊢< l > clam Mt ⇐ T ↣ lam_box t
+
+where "Γ ⊢< l > M ⇒ T ↣ t" := (infer Γ l M T t)
+and   "Γ ⊢< l > M ⇐ T ↣ t" := (check Γ l M T t).
+
+
+Scheme infer_mut := Induction for infer Sort Prop
+with check_mut := Induction for check Sort Prop.
+Combined Scheme infer_check_mutind from infer_mut, check_mut.
+
+
+Definition erase_ctx (Γ : ctx) := 
+    List.map (fun x => (fst x, erasure (Ax (fst x)) (snd x))) Γ.
+
+    
+Lemma var_in_erased_ctx Γ x l A : 
+    nth_error (erase_ctx Γ) x = Some (l, A) -> 
+    exists A', A = erasure (Ax l) A' /\ nth_error Γ x = Some (l, A').
+Proof.
+    intro H.
+    unfold erase_ctx in H.
+    rewrite nth_error_map in H.
+    destruct (nth_error Γ x); inversion H.
+    exists (snd p). split; eauto. destruct p; eauto.
+Qed.
+
+Lemma reduce_to_sort Γ l t A j :
+    Γ ⊢< l > t : A -> 
+    erasure (Ax l) A -->> Sort j -> 
+    Γ ⊢< Ax j > t : Sort j /\ l = Ax j.
+Proof.
+    intros t_Wt erasure_red.
+    eapply subject_reduction_redd in erasure_red as (_sort & TA_eq_sort & erasure_sort_eq_sort) ; eauto using validity_ty_ty.
+    destruct _sort; dependent destruction erasure_sort_eq_sort.
+    apply validity_conv_right in TA_eq_sort as Sort_wt. 
+    apply type_inv_sort' in Sort_wt as (_ & l_eq_0 & _).
+    apply Ax_inj in l_eq_0. dependent destruction l_eq_0.
+    split; eauto using type_conv.
+Qed.
+
+Lemma reduce_to_pi Γ l t T i j A B :
+    Γ ⊢< l > t : T -> 
+    erasure (Ax l) T -->> Pi i j A B -> 
+    exists A' B', A = erasure (Ax i) A' /\ B = erasure (Ax j) B' /\ Γ ⊢< Ru i j > t : Pi i j A' B' /\ l = Ru i j.
+Proof.
+    intros t_Wt erasure_red.
+    eapply subject_reduction_redd in erasure_red as (_pi & TA_eq_pi & erasure_pi_eq_pi) ; eauto using validity_ty_ty.
+    destruct _pi; dependent destruction erasure_pi_eq_pi.
+    apply validity_conv_right in TA_eq_pi as pi_wt. 
+    apply type_inv_pi' in pi_wt as (_ & _ & _ & l_eq_ru & _).
+    apply Ax_inj in l_eq_ru. dependent destruction l_eq_ru.
+    exists _pi1. exists _pi2.
+    split; eauto using type_conv.
+Qed.
+
+Lemma reduce_to_pi' Γ l T i j A B :
+    Γ ⊢< Ax l > T : Sort l -> 
+    erasure (Ax l) T -->> Pi i j A B -> 
+    exists A' B', A = erasure (Ax i) A' /\ B = erasure (Ax j) B' /\ Γ ⊢< Ax (Ru i j) > T ≡ Pi i j A' B' : Sort (Ru i j) /\ l = Ru i j.
+Proof.
+    intros t_Wt erasure_red.
+    eapply subject_reduction_redd in erasure_red as (_pi & TA_eq_pi & erasure_pi_eq_pi) ; eauto using validity_ty_ty.
+    destruct _pi; dependent destruction erasure_pi_eq_pi.
+    apply validity_conv_right in TA_eq_pi as pi_wt. 
+    apply type_inv_pi' in pi_wt as (_ & _ & _ & l_eq_ru & _).
+    apply Ax_inj in l_eq_ru. dependent destruction l_eq_ru.
+    exists _pi1. exists _pi2.
+    split; eauto using type_conv.
+Qed.
+
+
+Lemma reduce_to_nat Γ l t A :
+    Γ ⊢< l > t : A -> 
+    erasure (Ax l) A -->> Nat -> 
+    Γ ⊢< ty 0 > t : Nat /\ l = ty 0.
+Proof.
+    intros t_Wt erasure_red.
+    eapply subject_reduction_redd in erasure_red as (_nat & TA_eq_nat & erasure_nat_eq_nat) ; eauto using validity_ty_ty.
+    destruct _nat; dependent destruction erasure_nat_eq_nat.
+    apply validity_conv_right in TA_eq_nat as Nat_wt. 
+    apply type_inv_nat' in Nat_wt as (_ & l_eq_0 & _).
+    destruct l; inversion l_eq_0.
+    rewrite <- H0. eauto using type_conv.
+Qed.
+
+(* Lemma app_box_app Γ l A i t u :
+    Γ ⊢< l > t : A ->
+    app_box (erasure (ty i) t) u = app prop prop box box (erasure (ty i) t) u.
+Proof.
+    intro Wt.
+    destruct t; auto.
+    apply type_inv_box in Wt. inversion Wt.
+Qed. *)
+
+Lemma app_box_erasure Γ l T i j A B t u : 
+    Γ ⊢< l > t : T ->
+    erasure j (app i j A B t u) = app_box (erasure (Ru i j) t) (erasure i u).
+Proof.
+    intro H.
+    destruct j.
+    - simpl. destruct t; auto. apply type_inv_box in H. inversion H.
+    - repeat rewrite erasure_prop. auto.
+Qed. 
+
+Lemma lam_box_erasure Γ l T i j A B t : 
+    Γ ⊢< l > t : T ->
+    erasure (Ru i j) (lam i j A B t) = lam_box (erasure j t).
+Proof.
+    intro H.
+    destruct j.
+    - simpl. destruct t; auto. apply type_inv_box in H. inversion H.
+    - repeat rewrite erasure_prop. auto.
+Qed. 
+
+
+Lemma aux_subst_commute A l x Γ T : 
+    Γ ⊢< l > A : T ->
+    erasure l (A <[ succ (var x) .: ↑ >> (↑ >> var)]) = (erasure l A) <[ succ (var x) .: ↑ >> (↑ >> var)].
+Proof.
+    intro H.
+    setoid_rewrite (erasure_subst_commutes _ _ _ _ _ _ ((fun _ => ty 0) ;; (ty 0))).
+    setoid_rewrite erasure_cons. reflexivity. eauto. 
+    simpl.
+    assert (((λ _ : nat, ty 0);; ty 0) ~ fun _ => ty 0).
+    intro. destruct a; auto.
+    setoid_rewrite H0. 
+    apply refines_all.
+Qed.
+
+Theorem sound : 
+    (forall Γ l M T t, Γ ⊢< l > M ⇒ T ↣ t -> 
+        forall Γ' 
+        (erased_Γ'_eq : erase_ctx Γ' = Γ)
+        (Γ'Wf : ⊢ Γ'),
+        exists T' t', Γ' ⊢< l > t' : T' /\ erasure l t' = t /\ erasure (Ax l) T' = T
+    ) /\ (
+    forall Γ l M T t, Γ ⊢< l > M ⇐ T ↣ t -> 
+        forall Γ' T'
+        (erased_Γ'_eq : erase_ctx Γ' = Γ)
+        (erased_T'_eq : erasure (Ax l) T' = T)
+        (T'Wt : Γ' ⊢< Ax l > T' : Sort l),
+        exists t', Γ' ⊢< l > t' : T' /\ erasure l t' = t
+    ).
+Proof.
+    apply infer_check_mutind; intros; try rewrite <- erased_Γ'_eq in *; clear Γ erased_Γ'_eq.
+  
+    (* case var *)
+    - apply var_in_erased_ctx in e as (A' & H1 & H2). eexists. eexists. repeat split. 
+      eapply type_var; eauto. destruct l; auto. rewrite H1. apply erasure_rename_commute. 
+  
+    (* case sort *)
+    - eexists. exists (Sort l). split; eauto using type_sort.
+  
+    (* case Pi *)
+    - (* applying the ih to A *)
+      edestruct H as (TA & A' & A'_Wt & erased_A'_eq & erased_TA_eq); eauto.
+      dependent destruction erased_A'_eq. dependent destruction erased_TA_eq.
+      eapply reduce_to_sort in A'_Wt as (A'_Wt & _); eauto.
+      eapply type_conv in A'_Wt; eauto.
+      
+      (* applying the ih to B *)
+      edestruct (H0 (Γ' ,, (i, A'))) as (TB & B' & B'_Wt & erased_B'_eq & erased_TB_eq). 
+      all: (eauto using ctx_cons, conv_sort).
+      dependent destruction erased_B'_eq. dependent destruction erased_TB_eq.
+      eapply reduce_to_sort in B'_Wt as (B'_Wt & _); eauto.
+
+      exists (Sort (Ru i j)). exists (Pi i j A' B').
+      repeat split. auto using type_pi.
+
+    (* case app *)
+    - (* applying the ih to t *)
+      edestruct H as (A' & t' & t'_Wt & erasure_t'_eq & erasure_A'_eq); eauto.
+      dependent destruction erasure_t'_eq. dependent destruction erasure_A'_eq.
+      eapply reduce_to_pi in t'_Wt as (A0 & B0 & A_eq & B_eq & t'_Wt & l_eq); eauto.
+      dependent destruction A_eq. dependent destruction B_eq. dependent destruction l_eq.
+      apply validity_ty_ty in t'_Wt as PiA0B0_Wt. 
+      apply type_inv_pi' in PiA0B0_Wt as (_ & A0_Wt & B0_Wt & _ & _).
+
+      (* applying the ih to u *)
+      edestruct H0 as (u' & u'_Wt & erasure_u'_eq); eauto.
+      dependent destruction erasure_u'_eq.
+
+      exists (B0 <[ u' .. ]). exists (app i j A0 B0 t' u').
+      repeat split; eauto using type_app.
+      destruct j. 
+        + eapply app_box_erasure. eauto.
+        + simpl. rewrite erasure_prop. auto.
+        + eapply erasure_subst_1_commutes; eauto.
+    
+    (* case Nat *)
+    - eexists (Sort (ty 0)). eexists Nat. split; eauto using type_nat.
+
+    (* case zero *)
+    - eexists Nat. eexists zero. split; eauto using type_zero.
+
+    (* case succ *)
+    - (* applying the ih to t *)
+      edestruct H as (_Nat & t' & t'_Wt & erasure_t'_eq & erasure_Nat_eq); eauto.
+      dependent destruction erasure_t'_eq. dependent destruction erasure_Nat_eq.
+      eapply reduce_to_nat in t'_Wt as (t'_Wt & l_eq_0); eauto.
+      dependent destruction l_eq_0.
+      exists Nat. exists (succ t'). 
+      repeat split; eauto using type_succ.
+
+    (* case rec *)  
+    - (* applying the ih to P *)
+      edestruct (H (Γ' ,, (ty 0, Nat))) as (_sort & P' & P'_Wt & erased_P'_eq & erased_sort_eq); 
+      eauto using ctx_cons, type_nat.
+      dependent destruction erased_P'_eq. dependent destruction erased_sort_eq.
+      eapply reduce_to_sort in P'_Wt as (P'_Wt & l'_eq); eauto. dependent destruction l'_eq.
+      
+      (* applying the ih to p_zero *)
+      edestruct (H0 Γ' (P' <[ zero..])) as (p_zero' & p_zero'_Wt & erasure_eq); eauto.
+      eapply (erasure_subst_1_commutes _ (ty 0)); eauto.
+      eapply subst_ty'; eauto using aux_subst_1, type_zero.
+      dependent destruction erasure_eq.
+
+      (* applying the ih to p_succ *)
+      edestruct (H1 (Γ' ,, (ty 0, Nat) ,, (l, P')) (P' <[ succ (var 1) .: ↑ >> (↑ >> var)])) 
+        as (p_succ' & p_succ'_Wt & erasure_eq); eauto.
+      eapply aux_subst_commute; eauto.
+      eapply subst_ty'; eauto using aux_subst_2.
+      dependent destruction erasure_eq.
+      
+      (* applying the ih to k *)
+      edestruct (H2 Γ' Nat) as (k' & k'_Wt & erasure_eq); eauto using type_nat.
+      dependent destruction erasure_eq.
+
+      exists (P' <[ k' ..]). exists (rec l P' p_zero' p_succ' k').
+      repeat split.
+      auto using type_rec.
+      eapply erasure_subst_1_commutes; eauto.
+      
+    (* case annotation *)
+    - (* applying the ih to T *)
+      edestruct H as (_sort & T' & T'_Wt & erasure_T'_eq & erasure_sort_eq); eauto.
+      dependent destruction erasure_T'_eq. dependent destruction erasure_sort_eq.
+      eapply reduce_to_sort in T'_Wt as (T'_Wt & l_eq); eauto.
+      dependent destruction l_eq.
+
+      (* applying the ih to t *)
+      edestruct H0 as (t' & t'_Wt & erasure_t'_eq); eauto.
+      
+    (* case conv *)
+    - dependent destruction erased_T'_eq. 
+
+      (* applying the ih to t *)
+      edestruct H as (V' & t' & t'_Wt & erasure_t'_eq & erasure_V'_eq); eauto using validity_ty_ctx.
+      dependent destruction erasure_t'_eq. dependent destruction erasure_V'_eq.
+      eapply validity_ty_ty in t'_Wt as V'_Wt.
+      dependent destruction e.
+      assert (Γ' ⊢<Ax l > T'0 ≡ V' : Sort l) by (eapply convcheck_sound; eauto).
+      exists t'. split; eauto using type_conv, conv_sym.
+
+    (* case lam *)
+    - (* we first derive that T' is convertible to Pi A' B', 
+         and that A' B' are well-typed *)
+      dependent destruction erased_T'_eq. 
+      eapply reduce_to_pi' in T'Wt as (A' & B' & A_eq & B_eq & T'_eq & l_eq); eauto.
+      dependent destruction A_eq. dependent destruction B_eq. dependent destruction l_eq.
+      apply validity_conv_right in T'_eq as Pi_Wt.
+      apply type_inv_pi' in Pi_Wt as (_ & A'_Wt & B'_Wt & _).
+
+      (* applying the ih to t *)
+      edestruct H as (t' & t'_Wt & erased_t'_eq); eauto. 
+      unfold erase_ctx. reflexivity.
+      dependent destruction erased_t'_eq.
+
+      exists (lam i j A' B' t'). split; eauto using type_lam, type_conv, conv_sym, lam_box_erasure.      
+Qed.
+
+
+Corollary infer_sound Γ l M t T :
+    ⊢ Γ -> 
+    (erase_ctx Γ) ⊢< l > M ⇒ T ↣ t -> 
+    exists T' t', Γ ⊢< l > t' : T' /\ erasure l t' = t /\ erasure (Ax l) T' = T.
+Proof.
+    intros. eapply (proj1 sound); eauto.
+Qed.
+
+
+Corollary check_sound Γ l M t T :
+    Γ ⊢< Ax l > T : Sort l -> 
+    (erase_ctx Γ) ⊢< l > M ⇐ (erasure (Ax l) T) ↣ t -> 
+    exists t', Γ ⊢< l > t' : T /\ erasure l t' = t.
+Proof.
+    intros. eapply (proj2 sound); eauto.
+Qed.
